\documentclass[12pt]{article}
\usepackage{amssymb}
\usepackage{amsmath}

\title{MATH 330 -- HW \#29}
\author{Cristobal Forno}
\date{\today}

\begin{document}

\maketitle

\textbf{Question:} Let $z = x + yi$ be a complex number, where $x, y \in
\mathbb{R}$.
\newline
\textbf{(a)} $|\bar{z}| = |z|$.
\newline
\indent
\textbf{Proof:} We have the equation $|\bar{z}| = |z|$. If we square both sides,
we have $|\bar{z}|^2 = |z|^2$. This can be computed as $|x-yi|^2 = |x+yi|^2$,
where $x, y \in \mathbb{R}$. By Proposition C.9 (iii),
\begin{align}
  |x-yi|^2 &= (x+yi)(x-yi) \\
           &= x^2 + y^2 \\
           &= |x+yi| 
\end{align}
(3) is computed by the modulus of a complex number. Since $|x+yi| = |\bar{z}|$, we have prove
that $|z| = |\bar{z}|$. $\Box$


\noindent
\textbf{(b)} If $z \neq 0$, then $z^{-1} = \frac{\bar{z}}{|z|^2}$

\textbf{Proof:} Assume $z \neq 0$, where $z \in \mathbb{C}$. Let $z = x + yi$,
where $x, y \in \mathbb{R}$.Then there exists
an inverse of $z$, $z^{-1}$.
\begin{center}
$z^{-1} = \frac{1}{z} = \frac{\bar{z}}{z\bar{z}} = \frac{\bar{z}}{x^2+y^2} =
\frac{\bar{z}}{x^2 +(-1)y^2} =  \frac{\bar{z}}{x^2- y^2i^2} =
\frac{\bar{z}}{z^2} = \frac{\bar{z}}{|z|^2}$
\end{center}

The last equality is computed from Proposition 10.6. $\Box$
\end{document}